chore(data/nat/prime): style and minor modifications

data/nat/prime.lean
@@ -212,42 +212,38 @@ suffices ∀ {n}, n ≥ 2 → ∃ p, p ≥ n ∧ prime p, from
     pp.not_dvd_one this,
   ⟨p, this, pp⟩
 
+theorem factors_lemma {k} : (k+2) / min_fac (k+2) < k+2 :=
+div_lt_self dec_trivial (min_fac_prime dec_trivial).gt_one
+
 /-- `factors n` is the prime factorization of `n`, listed in increasing order. -/
 def factors : ℕ → list ℕ
 | 0 := []
 | 1 := []
-| n@(k+2) := let m := min_fac n in
-  have n / m < n, from
-    div_lt_self dec_trivial (min_fac_prime dec_trivial).gt_one,
+| n@(k+2) :=
+  let m := min_fac n in have n / m < n := factors_lemma,
   m :: factors (n / m)
 
 lemma mem_factors : ∀ {n p}, p ∈ factors n → prime p
-| 0       p h := absurd h (list.not_mem_nil _)
-| 1       p h := absurd h (list.not_mem_nil _)
-| n@(k+2) p h := 
-let m := min_fac n in
-have n / m < n, from
-  div_lt_self dec_trivial (min_fac_prime dec_trivial).gt_one,
-have h₁ : p = m ∨ p ∈ (factors (n / m)) := 
-  (list.mem_cons_iff _ _ _).1 h,
-or.cases_on h₁ (λ h₂, h₂.symm ▸ min_fac_prime dec_trivial)
-  mem_factors
-using_well_founded {rel_tac := λ _ _, `[exact ⟨_, measure_wf psigma.fst⟩]}
+| 0       := λ p, false.elim
+| 1       := λ p, false.elim
+| n@(k+2) := λ p h,
+  let m := min_fac n in have n / m < n := factors_lemma,
+  have h₁ : p = m ∨ p ∈ (factors (n / m)) := 
+    (list.mem_cons_iff _ _ _).1 h,
+  or.cases_on h₁ (λ h₂, h₂.symm ▸ min_fac_prime dec_trivial)
+    mem_factors
 
 lemma prod_factors : ∀ {n}, 0 < n → list.prod (factors n) = n 
-| 0       h := absurd h dec_trivial
-| 1       h := rfl
-| n@(k+2) h :=
-let m := min_fac n in
-have n / m < n, from
-  div_lt_self dec_trivial (min_fac_prime dec_trivial).gt_one,
-show list.prod (m :: factors (n / m)) = n, from
-have h₁ : 0 < n / m := 
-  nat.pos_of_ne_zero $ λ h,
-  have n = 0 * m := (nat.div_eq_iff_eq_mul_left (min_fac_pos _) (min_fac_dvd _)).1 h,
-  by rw zero_mul at this; exact (show k + 2 ≠ 0, from dec_trivial) this,
-by rw [list.prod_cons, prod_factors h₁, nat.mul_div_cancel' (min_fac_dvd _)]
-  using_well_founded {rel_tac := λ _ _, `[exact ⟨_, measure_wf psigma.fst⟩]}
+| 0       := (lt_irrefl _).elim
+| 1       := λ h, rfl
+| n@(k+2) := λ h,
+  let m := min_fac n in have n / m < n := factors_lemma,
+  show list.prod (m :: factors (n / m)) = n, from
+  have h₁ : 0 < n / m := 
+    nat.pos_of_ne_zero $ λ h,
+    have n = 0 * m := (nat.div_eq_iff_eq_mul_left (min_fac_pos _) (min_fac_dvd _)).1 h,
+    by rw zero_mul at this; exact (show k + 2 ≠ 0, from dec_trivial) this,
+  by rw [list.prod_cons, prod_factors h₁, nat.mul_div_cancel' (min_fac_dvd _)]
 
 theorem prime.coprime_iff_not_dvd {p n : ℕ} (pp : prime p) : coprime p n ↔ ¬ p ∣ n :=
 ⟨λ co d, pp.not_dvd_one $ co.dvd_of_dvd_mul_left (by simp [d]),
@@ -303,36 +299,34 @@ begin
       rw e, exact pow_dvd_pow _ l } }
 end
 
-end nat
-
-namespace nat
+section
 open list
 
 lemma mem_list_primes_of_dvd_prod {p : ℕ} (hp : prime p) : 
-    ∀ {l : list ℕ}, (∀ p ∈ l, prime p) → p ∣ prod l → p ∈ l
-| nil := λ h₁ h₂, absurd h₂ (prime.not_dvd_one hp)
+  ∀ {l : list ℕ}, (∀ p ∈ l, prime p) → p ∣ prod l → p ∈ l
+| []       := λ h₁ h₂, absurd h₂ (prime.not_dvd_one hp)
 | (q :: l) := λ h₁ h₂,
-have h₃ : p ∣ q * prod l := @prod_cons _ _ l q ▸ h₂,
-have hq : prime q := h₁ q (mem_cons_self _ _),
-or.cases_on ((prime.dvd_mul hp).1 h₃) 
-  (λ h, by rw [prime.dvd_iff_not_coprime hp, coprime_primes hp hq, ne.def, not_not] at h;
-    exact h ▸ mem_cons_self _ _) 
-  (λ h, have hl : ∀ p ∈ l, prime p := λ p hlp, h₁ p ((mem_cons_iff _ _ _).2 (or.inr hlp)),
-  (mem_cons_iff _ _ _).2 (or.inr (mem_list_primes_of_dvd_prod hl h)))
+  have h₃ : p ∣ q * prod l := @prod_cons _ _ l q ▸ h₂,
+  have hq : prime q := h₁ q (mem_cons_self _ _),
+  or.cases_on ((prime.dvd_mul hp).1 h₃) 
+    (λ h, by rw [prime.dvd_iff_not_coprime hp, coprime_primes hp hq, ne.def, not_not] at h;
+      exact h ▸ mem_cons_self _ _) 
+    (λ h, have hl : ∀ p ∈ l, prime p := λ p hlp, h₁ p ((mem_cons_iff _ _ _).2 (or.inr hlp)),
+    (mem_cons_iff _ _ _).2 (or.inr (mem_list_primes_of_dvd_prod hl h)))
 
 lemma mem_factors_of_dvd {n p : ℕ} (hn : 0 < n) (hp : prime p) (h : p ∣ n) : p ∈ factors n :=
 mem_list_primes_of_dvd_prod hp (@mem_factors n) ((prod_factors hn).symm ▸ h) 
 
-lemma perm_of_prod_eq_prod : ∀ {l₁ l₂ : list ℕ}, prod l₁ = prod l₂ → (∀ p ∈ l₁, prime p) →
-    (∀ p ∈ l₂, prime p) → l₁ ~ l₂
-| nil nil := λ _ _ _, perm.nil
-| nil (a :: l) := λ h₁ h₂ h₃,
+lemma perm_of_prod_eq_prod : ∀ {l₁ l₂ : list ℕ}, prod l₁ = prod l₂ →
+  (∀ p ∈ l₁, prime p) → (∀ p ∈ l₂, prime p) → l₁ ~ l₂
+| []        []        _  _  _  := perm.nil
+| []        (a :: l)  h₁ h₂ h₃ :=
   have ha : a ∣ 1 := @prod_nil ℕ _ ▸ h₁.symm ▸ (@prod_cons _ _ l a).symm ▸ dvd_mul_right _ _,
   absurd ha (prime.not_dvd_one (h₃ a (mem_cons_self _ _)))
-| (a :: l) nil := λ h₁ h₂ h₃,
+| (a :: l)  []        h₁ h₂ h₃ :=
   have ha : a ∣ 1 := @prod_nil ℕ _ ▸ h₁ ▸ (@prod_cons _ _ l a).symm ▸ dvd_mul_right _ _,
   absurd ha (prime.not_dvd_one (h₂ a (mem_cons_self _ _)))
-| (a :: l₁) (b :: l₂) := λ h hl₁ hl₂, 
+| (a :: l₁) (b :: l₂) h hl₁ hl₂ := 
   have hl₁' : ∀ p ∈ l₁, prime p := λ p hp, hl₁ p (mem_cons_of_mem _ hp),
   have hl₂' : ∀ p ∈ (b :: l₂).erase a, prime p := λ p hp, hl₂ p (mem_of_mem_erase hp),
   have ha : a ∈ (b :: l₂) := mem_list_primes_of_dvd_prod (hl₁ a (mem_cons_self _ _)) hl₂ 
@@ -344,14 +338,16 @@ lemma perm_of_prod_eq_prod : ∀ {l₁ l₂ : list ℕ}, prod l₁ = prod l₂ �
   perm.trans (perm.skip _ (perm_of_prod_eq_prod hl hl₁' hl₂')) hb.symm
 
 lemma factors_unique {n : ℕ} {l : list ℕ} (h₁ : prod l = n) (h₂ : ∀ p ∈ l, prime p) : l ~ factors n :=
-have hn : 0 < n := nat.pos_of_ne_zero (λ h, begin
-    rw h at *, clear h,
-    induction l with a l hi,
-    { exact absurd h₁ dec_trivial },
-    { rw prod_cons at h₁,
-      exact nat.mul_ne_zero (ne_of_lt (prime.pos (h₂ a (mem_cons_self _ _)))).symm
-        (hi (λ p hp, h₂ p (mem_cons_of_mem _ hp))) h₁ }
-  end),
+have hn : 0 < n := nat.pos_of_ne_zero $ λ h, begin
+  rw h at *, clear h,
+  induction l with a l hi,
+  { exact absurd h₁ dec_trivial },
+  { rw prod_cons at h₁,
+    exact nat.mul_ne_zero (ne_of_lt (prime.pos (h₂ a (mem_cons_self _ _)))).symm
+      (hi (λ p hp, h₂ p (mem_cons_of_mem _ hp))) h₁ }
+end,
 perm_of_prod_eq_prod (by rwa prod_factors hn) h₂ (@mem_factors _)
+
+end
 
 end nat
